Tweak setup of assumptions in top-level monotonicity result
Simplify instantiation by deferring the proof that the assumptions in
the fetch and execute phases evolve into each other, likely using system
invariants such as PCC always being unsealed.

model/Properties.thy
@@ -6,6 +6,10 @@ section \<open>Helper lemmas and definitions\<close>
 
 text \<open>TODO: Add to the Sail library\<close>
 
+lemma Traces_runTrace[simp]:
+  "(m, t, m') \<in> Traces \<Longrightarrow> runTrace t m = Some m'"
+  by (auto simp: runTrace_iff_Traces)
+
 fun consumesTrace :: "('regval, 'a, 'e) monad \<Rightarrow> 'regval trace \<Rightarrow> nat option" where
   "consumesTrace m [] = (if final m then Some 0 else None)"
 | "consumesTrace m (e # t) =
@@ -100,11 +104,9 @@ section \<open>Single-instruction monotonicity\<close>
 locale CHERI_ISA = Capability_Invariant_ISA CC ISA initial_caps cap_invariant
   for CC :: "'cap Capability_class" and ISA :: "('cap, 'regval, 'instr, 'e) isa"
     and cap_invariant :: "'cap \<Rightarrow> bool" and initial_caps :: "'cap set" +
-  fixes fetch_assms :: "'regval trace \<Rightarrow> bool" and instr_assms :: "'regval trace \<Rightarrow> bool"
-  assumes instr_cheri_axioms: "\<And>t n instr. hasTrace t \<lbrakk>instr\<rbrakk> \<Longrightarrow> n \<le> length t \<Longrightarrow> instr_available_caps_invariant instr t n \<Longrightarrow> instr_assms t \<Longrightarrow> instr_cheri_axioms instr t n"
+  fixes fetch_assms :: "'regval trace \<Rightarrow> bool" and instr_assms :: "'instr \<Rightarrow> 'regval trace \<Rightarrow> bool"
+  assumes instr_cheri_axioms: "\<And>t n instr. hasTrace t \<lbrakk>instr\<rbrakk> \<Longrightarrow> n \<le> length t \<Longrightarrow> instr_available_caps_invariant instr t n \<Longrightarrow> instr_assms instr t \<Longrightarrow> instr_cheri_axioms instr t n"
     and fetch_cheri_axioms: "\<And>t n. hasTrace t (instr_fetch ISA) \<Longrightarrow> n \<le> length t \<Longrightarrow> fetch_available_caps_invariant t n \<Longrightarrow> fetch_assms t \<Longrightarrow> fetch_cheri_axioms t n"
-    and instr_assms_appendE: "\<And>t t' instr. instr_assms (t @ t') \<Longrightarrow> Run \<lbrakk>instr\<rbrakk> t () \<Longrightarrow> instr_assms t \<and> fetch_assms t'"
-    and fetch_assms_appendE: "\<And>t t' instr. fetch_assms (t @ t') \<Longrightarrow> Run (instr_fetch ISA) t instr \<Longrightarrow> fetch_assms t \<and> instr_assms t'"
 
 locale Register_Accessors =
   fixes read_regval :: "register_name \<Rightarrow> 'regs \<Rightarrow> 'regval option"
@@ -118,11 +120,14 @@ abbreviation "s_allows_trace t s \<equiv> \<exists>s'. s_run_trace t s = Some s'
 end
 
 locale CHERI_ISA_State =
-  CHERI_ISA CC ISA cap_invariant initial_caps + Register_Accessors read_regval write_regval
-  for ISA :: "('cap, 'regval, 'instr, 'e) isa"
-  and CC :: "'cap Capability_class"
+  CHERI_ISA CC ISA cap_invariant initial_caps fetch_assms instr_assms +
+  Register_Accessors read_regval write_regval
+  for CC :: "'cap Capability_class"
+  and ISA :: "('cap, 'regval, 'instr, 'e) isa"
   and cap_invariant :: "'cap \<Rightarrow> bool"
   and initial_caps :: "'cap set"
+  and fetch_assms :: "'regval trace \<Rightarrow> bool"
+  and instr_assms :: "'instr \<Rightarrow> 'regval trace \<Rightarrow> bool"
   and read_regval :: "register_name \<Rightarrow> 'regs \<Rightarrow> 'regval option"
   and write_regval :: "register_name \<Rightarrow> 'regval \<Rightarrow> 'regs \<Rightarrow> 'regs option" +
   (* State versions of ISA model parameters *)
@@ -1031,7 +1036,7 @@ lemma hasTrace_instr_cheri_axioms:
   assumes t: "hasTrace t (instr_sem ISA instr)"
     and ci: "\<forall>c \<in> reachable_caps_plus C' s. is_tagged_method CC c \<longrightarrow> cap_invariant c"
     and initial_caps: "initial_caps \<subseteq> C'"
-    and ta: "instr_assms t"
+    and ta: "instr_assms instr t"
     and s': "s_run_trace (take n t) s = Some s'"
     and n: "n \<le> length t"
   shows "instr_cheri_axioms instr t n \<and> instr_available_caps_invariant instr t n"
@@ -1069,7 +1074,7 @@ lemma reachable_caps_plus_instr_trace_intradomain_monotonicity:
   assumes t: "hasTrace t (instr_sem ISA instr)"
     and ci: "\<forall>c \<in> reachable_caps_plus C'' s. is_tagged_method CC c \<longrightarrow> cap_invariant c"
     and initial_caps: "initial_caps \<subseteq> C''"
-    and ta: "instr_assms t"
+    and ta: "instr_assms instr t"
     and s': "s_run_trace t s = Some s'"
     and no_exception: "\<not>instr_raises_ex ISA instr t"
     and addr_trans_inv: "s_invariant_holds (addr_trans_invariant_plus C' False s) t s"
@@ -1090,7 +1095,7 @@ qed
 lemma reachable_caps_instr_trace_intradomain_monotonicity:
   assumes t: "hasTrace t (instr_sem ISA instr)"
     and ci: "\<forall>c \<in> reachable_caps s. is_tagged_method CC c \<longrightarrow> cap_invariant c"
-    and ta: "instr_assms t"
+    and ta: "instr_assms instr t"
     and s': "s_run_trace t s = Some s'"
     and no_exception: "\<not>instr_raises_ex ISA instr t"
     and invoked_caps_reachable: "invoked_instr_caps instr t \<subseteq> reachable_caps s"
@@ -1292,6 +1297,15 @@ declare instrs_raise_ex.simps[simp del]
 context CHERI_ISA_State
 begin
 
+fun instrs_assms :: "nat \<Rightarrow> 'regval trace \<Rightarrow> bool" where
+  "instrs_assms (Suc n) t =
+     (\<forall>nf. consumesTrace (instr_fetch ISA) t = Some nf
+       \<longrightarrow> fetch_assms (take nf t)
+         \<and> (\<forall>instr ni. runTrace (take nf t) (instr_fetch ISA) = Some (Done instr)
+                     \<and> consumesTrace (instr_sem ISA instr) (drop nf t) = Some ni
+                    \<longrightarrow> instr_assms instr (take ni (drop nf t)) \<and> instrs_assms n (drop (nf + ni) t)))"
+| "instrs_assms 0 t = True"
+
 abbreviation "invoked_instrs_caps n t \<equiv> instrs_invoke_caps ISA n t \<union> instrs_invoke_indirect_caps ISA n t"
 
 lemma invoked_instrs_caps_Suc:
@@ -1304,7 +1318,7 @@ lemma invoked_instrs_caps_Suc:
 lemma reachable_caps_plus_instrs_trace_intradomain_monotonicity:
   assumes t: "hasTrace t (fetch_execute_loop ISA n)"
     and ci: "\<forall>c \<in> reachable_caps_plus (initial_caps \<union> invoked_instrs_caps n t) s. is_tagged_method CC c \<longrightarrow> cap_invariant c"
-    and ta: "fetch_assms t"
+    and ta: "instrs_assms n t"
     and s': "s_run_trace t s = Some s'"
     and no_exception: "\<not>instrs_raise_ex ISA n t"
     and addr_trans_inv: "s_invariant_holds (addr_trans_invariant_plus (initial_caps \<union> invoked_instrs_caps n t) False s) t s"
@@ -1331,6 +1345,7 @@ next
       by (elim s_invariant_holds_weaken) (auto intro: addr_trans_invariant_plus_antimono)
     ultimately have "reachable_caps_plus {} s' \<subseteq> reachable_caps_plus ({} \<union> initial_caps) s"
       using Suc.prems fetch_raises_ex_instrs_raise_ex[where tf = t and t' = "[]"]
+      using hasTrace_consumesTrace[where t = t and t' = "[]" and m = "instr_fetch ISA"]
       by (intro reachable_caps_plus_fetch_trace_intradomain_monotonicity) auto
     also have "\<dots> \<subseteq> reachable_caps_plus (initial_caps \<union> invoked_instrs_caps (Suc n) t) s"
       by (intro reachable_caps_plus_mono) auto
@@ -1348,9 +1363,9 @@ next
     have no_fetch_ex: "\<not>fetch_raises_ex ISA tf"
       using Suc.prems \<open>t = tf @ t'\<close>
       by auto
-    have ta': "fetch_assms tf" "instr_assms t'"
-      using Bind Suc.prems fetch_assms_appendE
-      by auto
+    have ta': "fetch_assms tf"
+      using Bind \<open>instrs_assms (Suc n) t\<close>
+      by (auto simp: Run_hasTrace[THEN hasTrace_consumesTrace])
     have fetch_mono: "reachable_caps_plus (initial_caps \<union> invoked_instrs_caps (Suc n) t) s'' \<subseteq> reachable_caps_plus (initial_caps \<union> invoked_instrs_caps (Suc n) t) s"
       using tf s'' Bind Suc.prems ta'
       by (intro reachable_caps_plus_fetch_trace_intradomain_monotonicity)
@@ -1370,13 +1385,16 @@ next
       then have *: "hasTrace t' \<lbrakk>instr\<rbrakk>"
         using m'
         by (auto elim!: final_bind_cases) (auto simp: hasTrace_iff_Traces_final final_def)
+      have ta'': "instr_assms instr t'"
+        using Bind \<open>instrs_assms (Suc n) t\<close> hasTrace_consumesTrace[where t' = "[]", OF *]
+        by (auto simp: Run_hasTrace[THEN hasTrace_consumesTrace])
       have inv'': "s_invariant_holds (addr_trans_invariant_plus ({} \<union> initial_caps \<union> invoked_instr_caps instr t') False s'') t' s''"
         using inv' \<open>t = tf @ t'\<close>
         using instrs_invoke_caps_Suc[OF \<open>Run (instr_fetch ISA) tf instr\<close> *, where t' = "[]"]
         using instrs_invoke_indirect_caps_Suc[OF \<open>Run (instr_fetch ISA) tf instr\<close> *, where t' = "[]"]
         by (elim s_invariant_holds_weaken addr_trans_invariant_plus_antimono) auto
       have "reachable_caps_plus {} s' \<subseteq> reachable_caps_plus ({} \<union> initial_caps \<union> invoked_instr_caps instr t') s''"
-        using * tf t' s'' Bind Suc.prems inv'' ta' fetch_cap_inv
+        using * tf t' s'' Bind Suc.prems inv'' ta'' fetch_cap_inv
         using instrs_raise_ex_Suc[OF \<open>Run (instr_fetch ISA) tf instr\<close> *, where t' = "[]"]
         by (intro reachable_caps_plus_instr_trace_intradomain_monotonicity)
            (auto simp add: runTrace_iff_Traces)
@@ -1393,9 +1411,9 @@ next
       have ti: "hasTrace ti \<lbrakk>instr\<rbrakk>"
         using Bind
         by (auto simp: hasTrace_iff_Traces_final final_def)
-      have ta'': "instr_assms ti" "fetch_assms t''"
-        using Bind ta' instr_assms_appendE
-        by auto
+      have ta'': "instr_assms instr ti" "instrs_assms n t''"
+        using Bind \<open>Run (instr_fetch ISA) tf instr\<close> \<open>t = tf @ t'\<close> \<open>instrs_assms (Suc n) t\<close>
+        by (auto simp: Run_hasTrace[THEN hasTrace_consumesTrace])
       have no_exception': "\<not>fetch_raises_ex ISA tf" "\<not>instr_raises_ex ISA instr ti"
         and no_exception'': "\<not>instrs_raise_ex ISA n t''"
         using ti tf Suc.prems Bind \<open>t = tf @ t'\<close>
@@ -1432,7 +1450,7 @@ qed
 lemma reachable_caps_instrs_trace_intradomain_monotonicity:
   assumes t: "hasTrace t (fetch_execute_loop ISA n)"
     and ci: "\<forall>c \<in> reachable_caps s. is_tagged_method CC c \<longrightarrow> cap_invariant c"
-    and ta: "fetch_assms t"
+    and ta: "instrs_assms n t"
     and s': "s_run_trace t s = Some s'"
     and no_exception: "\<not>instrs_raise_ex ISA n t"
     and invoked_caps_reachable: "invoked_instrs_caps n t \<subseteq> reachable_caps s"
@@ -1445,7 +1463,6 @@ proof -
     by simp
   note [simp] = reachable_caps_plus_subset_eq[OF this] addr_trans_invariant_plus_subset_reachable_caps_eq[OF this]
   from assms have "reachable_caps s' \<subseteq> reachable_caps_plus (initial_caps \<union> invoked_instrs_caps n t) s"
-    thm reachable_caps_plus_instrs_trace_intradomain_monotonicity
     by (intro reachable_caps_plus_instrs_trace_intradomain_monotonicity) auto
   then show ?thesis
     by simp
